src/Minimal.DICE.fst
@@ -24,6 +24,7 @@ module HS  = FStar.HyperStack
 module HST = FStar.HyperStack.ST
 module IB  = LowStar.ImmutableBuffer
 
+inline_for_extraction
 let dice_hash (alg: dice_alg): hash_st alg =
   match alg with
   | SHA2_256 -> SHA2.hash_256
@@ -31,14 +32,13 @@ let dice_hash (alg: dice_alg): hash_st alg =
   | SHA2_512 -> SHA2.hash_512
   | SHA1     -> SHA1.legacy_hash
 
+inline_for_extraction
 let dice_hmac (alg: dice_alg): HMAC.compute_st alg =
   match alg with
   | SHA2_256 -> HMAC.compute_sha2_256
   | SHA2_384 -> HMAC.compute_sha2_384
   | SHA2_512 -> HMAC.compute_sha2_512
   | SHA1     -> HMAC.legacy_compute_sha1
-
-let (++) = List.append
 
 /// compute digest of `uds`
 let compute_uDigest
@@ -63,21 +63,22 @@ let compute_uDigest
 /// compute measurement of RIoT firmware
 let compute_rDigest
   (rDigest: B.buffer uint8{B.length rDigest == hash_length alg})
-  (riot: riot_t)
+  (riot_size: riot_size_t)
+  (riot_binary: B.buffer uint8 {B.length riot_binary == v riot_size})
 : HST.StackInline unit
   (requires fun h ->
-      B.all_live h [B.buf riot.binary
+      B.all_live h [B.buf riot_binary
                    ;B.buf rDigest]
-    /\ B.all_disjoint [B.loc_buffer riot.binary
+    /\ B.all_disjoint [B.loc_buffer riot_binary
                      ;B.loc_buffer rDigest])
   (ensures  fun h0 _ h1 ->
       B.modifies (B.loc_buffer rDigest) h0 h1
     /\ B.as_seq h1 rDigest
-      == Spec.Agile.Hash.hash alg (B.as_seq h0 riot.binary))
+      == Spec.Agile.Hash.hash alg (B.as_seq h0 riot_binary))
 =
   dice_hash alg
-    riot.binary
-    riot.size
+    riot_binary
+    riot_size
     rDigest
 
 
@@ -99,6 +100,8 @@ let compute_cdi
     /\ B.as_seq h1 cdi
       == Spec.Agile.HMAC.hmac alg (B.as_seq h0 uDigest) (B.as_seq h0 rDigest))
 =
+  (**)let h = HST.get() in
+  (**)assert (Spec.Agile.HMAC.keysized alg (Seq.length (B.as_seq h uDigest)));
   dice_hmac alg
     cdi
     uDigest (hash_len alg)
@@ -115,20 +118,23 @@ let compute_cdi
 #reset-options "--z3rlimit 30"
 let dice_on_stack
   (st: state)
+  (riot_size: riot_size_t)
+  (riot_binary: B.buffer uint8 {B.length riot_binary == v riot_size})
 : HST.Stack unit
   (requires fun h ->
-      B.all_live h (get_buf_t_l st)
-    /\ B.all_disjoint (get_loc_l st))
+    h `HWIface.contains` st /\
+    h `B.live` riot_binary /\
+    B.all_disjoint ((get_loc_l st)@[B.loc_buffer riot_binary]))
   (ensures  fun h0 _ h1 ->
-    let uds, cdi, riot = get_uds st, get_cdi st, get_riot st in
-      B.modifies (B.loc_buffer cdi) h0 h1
-    /\ B.as_seq h1 cdi
-      == Spec.Agile.HMAC.hmac alg
-           (Spec.Agile.Hash.hash alg (B.as_seq h0 uds))
-           (Spec.Agile.Hash.hash alg (B.as_seq h0 riot.binary)))
+    let uds, cdi = get_uds st, get_cdi st in
+      B.modifies (B.loc_buffer cdi) h0 h1 /\
+      B.as_seq h1 cdi
+        == Spec.Agile.HMAC.hmac alg
+             (Spec.Agile.Hash.hash alg (B.as_seq h0 uds))
+             (Spec.Agile.Hash.hash alg (B.as_seq h0 riot_binary)))
 =
   HST.push_frame();
-  let uds, cdi, riot = get_uds st, get_cdi st, get_riot st in
+  let uds, cdi = get_uds st, get_cdi st in
 
   (* compute digest of `uds` *)
   let uDigest: b:B.buffer uint8{B.length b == hash_length alg}
@@ -138,10 +144,13 @@ let dice_on_stack
   (* compute measurement of RIoT firmware *)
   let rDigest: b:B.buffer uint8{B.length b == hash_length alg}
     = B.alloca (u8 0x00) digest_length
-  in compute_rDigest rDigest riot;
+  in compute_rDigest rDigest riot_size riot_binary;
 
   (* compute `cdi` *)
-  compute_cdi cdi uDigest rDigest;
+  dice_hmac alg
+    cdi
+    uDigest (hash_len alg)
+    rDigest (hash_len alg);
 
   HST.pop_frame()
 
@@ -152,21 +161,27 @@ let dice_on_stack
 #reset-options "--z3rlimit 30"
 let dice_main
   (riot_size: riot_size_t)
+  (riot_binary: B.buffer uint8 {B.length riot_binary == v riot_size})
 : HST.ST unit
   (requires fun h ->
-      uds_is_uninitialized h)
-  (ensures  fun h0 _ h1 ->
-      uds_is_disabled)
+    uds_is_uninitialized h /\
+    h `B.live` riot_binary)
+  (ensures  fun h0 _ h1 -> uds_is_disabled)
 =
   (* allocating in the heap *)
-  let st = initialize riot_size in
+  let st = initialize () in
+  let h = HST.get () in
+  assert (B.disjoint (get_uds st) riot_binary);
+  st
 
   (* only allocating on the stack *)
-  dice_on_stack st;
+  dice_on_stack st riot_size riot_binary;
 
   (* wipe and disable uds *)
   unset_uds st;
-  disable_uds st
+  disable_uds st;
+
+  st
 
 /// <><><><><><><><><><><><> C main funtion <><><><><><><><><><><>
 
